feat: lemmas about iterator collectors (#8380)
This PR provides simple lemmas about `toArray`, `toList` and `toListRev`
for the iterator library.

It also changes the definition of `Iter` and `IterM` so that they aren't
equal anymore and in particular not definitionally equal. While it was
very convenient to have them be definitionally equal when working with
dependent code, it was also confusing and annoying that one would
sometimes end up with something like `it.toList = IterM.toList it`,
where `it : Iter β`.

src/Std/Data/Iterators/Basic.lean
@@ -20,16 +20,6 @@ namespace Std
 namespace Iterators
 
 /--
-`BaseIter` is the common data structure underlying `Iter` and `IterM`. API users should never
-use `BaseIter` directly, only `Iter` and `IterM`.
--/
-structure BaseIter {α : Type w} (m : Type w → Type w') (β : Type w) : Type w where
-  /--
-  Internal implementation detail of the iterator.
-  -/
-  internalState : α
-
-/--
 An iterator that sequentially emits values of type `β` in the monad `m`. It may be finite
 or infinite.
 
@@ -68,7 +58,9 @@ def x := [1, 2, 3].iterM IO
 def x := ([1, 2, 3].iterM IO : IterM IO Nat)
 ```
 -/
-def IterM {α : Type w} (m : Type w → Type w') (β : Type w) := BaseIter (α := α) m β
+structure IterM {α : Type w} (m : Type w → Type w') (β : Type w) where
+  /-- Internal implementation detail of the iterator. -/
+  internalState : α
 
 /--
 An iterator that sequentially emits values of type `β`. It may be finite
@@ -109,29 +101,41 @@ def x := [1, 2, 3].iter
 def x := ([1, 2, 3].iter : Iter Nat)
 ```
 -/
-def Iter {α : Type w} (β : Type w) := BaseIter (α := α) Id β
+structure Iter {α : Type w} (β : Type w) where
+  /-- Internal implementation detail of the iterator. -/
+  internalState : α
 
 /--
 Converts a pure iterator (`Iter β`) into a monadic iterator (`IterM Id β`) in the
 identity monad `Id`.
 -/
 def Iter.toIterM {α : Type w} {β : Type w} (it : Iter (α := α) β) : IterM (α := α) Id β :=
-  it
+  ⟨it.internalState⟩
 
 /--
 Converts a monadic iterator (`IterM Id β`) over `Id` into a pure iterator (`Iter β`).
 -/
-def IterM.toPureIter {α : Type w} {β : Type w} (it : IterM (α := α) Id β) : Iter (α := α) β :=
-  it
+def IterM.toIter {α : Type w} {β : Type w} (it : IterM (α := α) Id β) : Iter (α := α) β :=
+  ⟨it.internalState⟩
 
 @[simp]
-theorem Iter.toPureIter_toIterM {α : Type w} {β : Type w} (it : Iter (α := α) β) :
-    it.toIterM.toPureIter = it :=
+theorem Iter.toIter_toIterM {α : Type w} {β : Type w} (it : Iter (α := α) β) :
+    it.toIterM.toIter = it :=
   rfl
 
 @[simp]
-theorem Iter.toIterM_toPureIter {α : Type w} {β : Type w} (it : IterM (α := α) Id β) :
-    it.toPureIter.toIterM = it :=
+theorem Iter.toIter_comp_toIterM {α : Type w} {β : Type w} :
+    IterM.toIter ∘ Iter.toIterM (α := α) (β := β) = id :=
+  rfl
+
+@[simp]
+theorem Iter.toIterM_toIter {α : Type w} {β : Type w} (it : IterM (α := α) Id β) :
+    it.toIter.toIterM = it :=
+  rfl
+
+@[simp]
+theorem Iter.toIterM_comp_toIter {α : Type w} {β : Type w} :
+    Iter.toIterM ∘ IterM.toIter (α := α) (β := β) = id :=
   rfl
 
 section IterStep
@@ -170,6 +174,27 @@ def IterStep.successor : IterStep α β → Option α
   | .done => none
 
 /--
+If present, applies `f` to the iterator of an `IterStep` and replaces the iterator
+with the result of the application of `f`.
+-/
+@[always_inline, inline]
+def IterStep.mapIterator {α' : Type u'} (f : α → α') : IterStep α β → IterStep α' β
+  | .yield it out => .yield (f it) out
+  | .skip it => .skip (f it)
+  | .done => .done
+
+@[simp]
+theorem IterStep.mapIterator_mapIterator {α' : Type u'} {α'' : Type u''}
+    {f : α → α'} {g : α' → α''} {step : IterStep α β} :
+    (step.mapIterator f).mapIterator g = step.mapIterator (g ∘ f) := by
+  cases step <;> rfl
+
+@[simp]
+theorem IterStep.mapIterator_id {step : IterStep α β} :
+    step.mapIterator id = step := by
+  cases step <;> rfl
+
+/--
 A variant of `IterStep` that bundles the step together with a proof that it is "plausible".
 The plausibility predicate will later be chosen to assert that a state is a plausible successor
 of another state. Having this proof bundled up with the step is important for termination proofs.
@@ -202,6 +227,20 @@ Match pattern for the `done` case. See also `IterStep.done`.
 def PlausibleIterStep.done {IsPlausibleStep : IterStep α β → Prop}
     (h : IsPlausibleStep .done) : PlausibleIterStep IsPlausibleStep :=
   ⟨.done, h⟩
+
+/--
+A more convenient `cases` eliminator for `PlausibleIterStep`.
+-/
+@[elab_as_elim, cases_eliminator]
+abbrev PlausibleIterStep.casesOn {IsPlausibleStep : IterStep α β → Prop}
+    {motive : PlausibleIterStep IsPlausibleStep → Sort x} (s : PlausibleIterStep IsPlausibleStep)
+    (yield : ∀ it' out h, motive ⟨.yield it' out, h⟩)
+    (skip : ∀ it' h, motive ⟨.skip it', h⟩)
+    (done : ∀ h, motive ⟨.done, h⟩) : motive s :=
+  match s with
+  | .yield it' out h => yield it' out h
+  | .skip it' h => skip it' h
+  | .done h => done h
 
 end IterStep
 
@@ -296,7 +335,7 @@ is up to the `Iterator` instance but it should be strong enough to allow termina
 -/
 def Iter.IsPlausibleStep {α : Type w} {β : Type w} [Iterator α Id β]
     (it : Iter (α := α) β) (step : IterStep (Iter (α := α) β) β) : Prop :=
-  it.toIterM.IsPlausibleStep step
+  it.toIterM.IsPlausibleStep (step.mapIterator Iter.toIterM)
 
 /--
 The type of the step object returned by `Iter.step`, containing an `IterStep`
@@ -304,6 +343,37 @@ and a proof that this is a plausible step for the given iterator.
 -/
 def Iter.Step {α : Type w} {β : Type w} [Iterator α Id β] (it : Iter (α := α) β) :=
   PlausibleIterStep (Iter.IsPlausibleStep it)
+
+/--
+Converts an `Iter.Step` into an `IterM.Step`.
+-/
+@[always_inline, inline]
+def Iter.Step.toMonadic {α : Type w} {β : Type w} [Iterator α Id β] {it : Iter (α := α) β}
+    (step : it.Step) : it.toIterM.Step :=
+  ⟨step.val.mapIterator Iter.toIterM, step.property⟩
+
+/--
+Converts an `IterM.Step` into an `Iter.Step`.
+-/
+@[always_inline, inline]
+def IterM.Step.toPure {α : Type w} {β : Type w} [Iterator α Id β] {it : IterM (α := α) Id β}
+    (step : it.Step) : it.toIter.Step :=
+  ⟨step.val.mapIterator IterM.toIter, (by simp [Iter.IsPlausibleStep, step.property])⟩
+
+@[simp]
+theorem IterM.Step.toPure_yield {α β : Type w} [Iterator α Id β] {it : IterM (α := α) Id β}
+    {it' out h} : IterM.Step.toPure (⟨.yield it' out, h⟩ : it.Step) = .yield it'.toIter out h :=
+  rfl
+
+@[simp]
+theorem IterM.Step.toPure_skip {α β : Type w} [Iterator α Id β] {it : IterM (α := α) Id β}
+    {it' h} : IterM.Step.toPure (⟨.skip it', h⟩ : it.Step) = .skip it'.toIter h :=
+  rfl
+
+@[simp]
+theorem IterM.Step.toPure_done {α β : Type w} [Iterator α Id β] {it : IterM (α := α) Id β}
+    {h} : IterM.Step.toPure (⟨.done, h⟩ : it.Step) = .done h :=
+  rfl
 
 /--
 Asserts that a certain output value could plausibly be emitted by the given iterator in its next
@@ -319,7 +389,7 @@ given iterator `it`.
 -/
 def Iter.IsPlausibleSuccessorOf {α : Type w} {β : Type w} [Iterator α Id β]
     (it' it : Iter (α := α) β) : Prop :=
-  it'.toIterM.IsPlausibleSuccessorOf it
+  it'.toIterM.IsPlausibleSuccessorOf it.toIterM
 
 /--
 Asserts that a certain iterator `it'` could plausibly be the directly succeeding iterator of another
@@ -327,7 +397,7 @@ given iterator `it` while no value is emitted (see `IterStep.skip`).
 -/
 def Iter.IsPlausibleSkipSuccessorOf {α : Type w} {β : Type w} [Iterator α Id β]
     (it' it : Iter (α := α) β) : Prop :=
-  it'.toIterM.IsPlausibleSkipSuccessorOf it
+  it'.toIterM.IsPlausibleSkipSuccessorOf it.toIterM
 
 /--
 Makes a single step with the given iterator `it`, potentially emitting a value and providing a
@@ -336,7 +406,7 @@ the termination measures `it.finitelyManySteps` and `it.finitelyManySkips`.
 -/
 @[always_inline, inline]
 def Iter.step {α β : Type w} [Iterator α Id β] (it : Iter (α := α) β) : it.Step :=
-  it.toIterM.step
+  it.toIterM.step.run.toPure
 
 end Pure
 
@@ -415,14 +485,14 @@ with `IterM.finitelyManySteps`.
 theorem Iter.TerminationMeasures.Finite.rel_of_yield
     {α : Type w} {β : Type w} [Iterator α Id β]
     {it it' : Iter (α := α) β} {out : β} (h : it.IsPlausibleStep (.yield it' out)) :
-    IterM.TerminationMeasures.Finite.Rel ⟨it'⟩ ⟨it⟩ :=
+    IterM.TerminationMeasures.Finite.Rel ⟨it'.toIterM⟩ ⟨it.toIterM⟩ :=
   IterM.TerminationMeasures.Finite.rel_of_yield h
 
 @[inherit_doc Iter.TerminationMeasures.Finite.rel_of_yield]
 theorem Iter.TerminationMeasures.Finite.rel_of_skip
     {α : Type w} {β : Type w} [Iterator α Id β]
     {it it' : Iter (α := α) β} (h : it.IsPlausibleStep (.skip it')) :
-    IterM.TerminationMeasures.Finite.Rel ⟨it'⟩ ⟨it⟩ :=
+    IterM.TerminationMeasures.Finite.Rel ⟨it'.toIterM⟩ ⟨it.toIterM⟩ :=
   IterM.TerminationMeasures.Finite.rel_of_skip h
 
 macro_rules | `(tactic| decreasing_trivial) => `(tactic|
